src/concurrency/DNS.ShellResponseBoundary.fst
@@ -7,6 +7,7 @@ module COMPLETE = DNS.QUIC.MsQuicSendCompletion
 module EGRESS = DNS.QUIC.MsQuicEgress
 module MUX = DNS.QUIC.Multiplexer
 module STREAM = DNS.QUIC.StreamMapping
+module CAST = FStar.Int.Cast
 
 (* C-facing response boundary for the unverified shell. The shell provides a
    response buffer already filled by verified response construction and receives
@@ -39,6 +40,107 @@ let prepare_response_send_for_stream ctx_ptr response_buffer response_len fin_co
   } in
   let descriptor = EGRESS.prepare_response_send () ctx_ptr response in
   descriptor.EGRESS.mssd_len
+
+val copy_response_bytes_with_prefix :
+  response_buffer:buffer FStar.UInt8.t ->
+  stream_buffer:buffer FStar.UInt8.t ->
+  response_len:FStar.UInt32.t ->
+  idx:FStar.UInt32.t{FStar.UInt32.v idx <= FStar.UInt32.v response_len} ->
+  ST unit
+    (requires (fun h0 ->
+      live h0 response_buffer /\
+      live h0 stream_buffer /\
+      FStar.UInt32.v response_len <= 65535 /\
+      FStar.UInt32.v response_len <= LowStar.Buffer.length response_buffer /\
+      FStar.UInt32.v response_len + 2 <= LowStar.Buffer.length stream_buffer))
+    (ensures (fun h0 _ h1 ->
+      modifies (loc_buffer stream_buffer) h0 h1 /\
+      live h1 stream_buffer))
+    (decreases (FStar.UInt32.v response_len - FStar.UInt32.v idx))
+
+let rec copy_response_bytes_with_prefix response_buffer stream_buffer response_len idx =
+  if FStar.UInt32.eq idx response_len then
+    ()
+  else
+    begin
+      assert (FStar.UInt32.v idx < FStar.UInt32.v response_len);
+      assert (FStar.UInt32.v idx < 65535);
+      assert (2 + FStar.UInt32.v idx < 4294967296);
+      let dst_idx = FStar.UInt32.add 2ul idx in
+      assert (FStar.UInt32.v idx < LowStar.Buffer.length response_buffer);
+      assert (FStar.UInt32.v dst_idx < LowStar.Buffer.length stream_buffer);
+      let byte = LowStar.Buffer.index response_buffer idx in
+      LowStar.Buffer.upd stream_buffer dst_idx byte;
+      assert (FStar.UInt32.v idx + 1 <= FStar.UInt32.v response_len);
+      assert (FStar.UInt32.v idx + 1 < 4294967296);
+      let next_idx = FStar.UInt32.add idx 1ul in
+      assert (FStar.UInt32.v next_idx = FStar.UInt32.v idx + 1);
+      copy_response_bytes_with_prefix response_buffer stream_buffer response_len next_idx
+    end
+
+val prepare_doq_response_send_for_stream :
+  ctx_ptr:buffer STREAM.stream_context ->
+  response_buffer:buffer FStar.UInt8.t ->
+  response_len:FStar.UInt32.t ->
+  stream_buffer:buffer FStar.UInt8.t ->
+  stream_capacity:FStar.UInt32.t ->
+  fin_code:FStar.UInt8.t ->
+  ST FStar.UInt32.t
+    (requires (fun h0 ->
+      live h0 ctx_ptr /\
+      LowStar.Buffer.length ctx_ptr >= 1 /\
+      live h0 response_buffer /\
+      live h0 stream_buffer /\
+      FStar.UInt32.v response_len <= LowStar.Buffer.length response_buffer /\
+      FStar.UInt32.v stream_capacity <= LowStar.Buffer.length stream_buffer /\
+      loc_disjoint (loc_buffer ctx_ptr) (loc_buffer stream_buffer) /\
+      loc_disjoint (loc_buffer response_buffer) (loc_buffer stream_buffer) /\
+      (let ctx = FStar.Seq.index (LowStar.Buffer.as_seq h0 ctx_ptr) 0 in
+       live h0 ctx.STREAM.sc_buf)))
+    (ensures (fun h0 _ h1 ->
+      modifies (loc_buffer stream_buffer) h0 h1 /\
+      live h1 stream_buffer))
+
+let prepare_doq_response_send_for_stream
+  ctx_ptr
+  response_buffer
+  response_len
+  stream_buffer
+  stream_capacity
+  fin_code =
+  if FStar.UInt32.gt response_len 65535ul then
+    0ul
+  else
+    begin
+      assert (FStar.UInt32.v response_len <= 65535);
+      assert (FStar.UInt32.v response_len + 2 < 4294967296);
+      let framed_len = FStar.UInt32.add response_len 2ul in
+      if FStar.UInt32.lt stream_capacity framed_len then
+        0ul
+      else
+        begin
+          assert (FStar.UInt32.v framed_len <= FStar.UInt32.v stream_capacity);
+          assert (FStar.UInt32.v framed_len <= LowStar.Buffer.length stream_buffer);
+          assert (2 <= LowStar.Buffer.length stream_buffer);
+          assert (0 < LowStar.Buffer.length stream_buffer);
+          assert (1 < LowStar.Buffer.length stream_buffer);
+          let s = LowStar.Buffer.index ctx_ptr 0ul in
+          let hi32 = FStar.UInt32.shift_right response_len 8ul in
+          let len_hi = CAST.uint32_to_uint8 hi32 in
+          let len_lo = CAST.uint32_to_uint8 response_len in
+          LowStar.Buffer.upd stream_buffer 0ul len_hi;
+          LowStar.Buffer.upd stream_buffer 1ul len_lo;
+          copy_response_bytes_with_prefix response_buffer stream_buffer response_len 0ul;
+          let response = {
+            EGRESS.msrf_stream_id = s.STREAM.sc_id;
+            EGRESS.msrf_data = stream_buffer;
+            EGRESS.msrf_len = framed_len;
+            EGRESS.msrf_fin = not (FStar.UInt8.eq fin_code 0uy);
+          } in
+          let descriptor = EGRESS.prepare_response_send () ctx_ptr response in
+          descriptor.EGRESS.mssd_len
+        end
+    end
 
 val send_outcome_of_code :
   code:FStar.UInt8.t ->
